theories/typing.v
@@ -197,10 +197,9 @@ Inductive be_typing : t_context -> seq basic_instruction -> function_type -> Pro
 | bet_testop : forall C t op, is_int_t t -> be_typing C [::BI_testop t op] (Tf [::T_num t] [::T_num T_i32])
 | bet_relop: forall C t op,
     relop_type_agree t op -> be_typing C [::BI_relop t op] (Tf [::T_num t; T_num t] [::T_num T_i32])
-| bet_convert : forall C t1 t2 sx, t1 <> t2 -> convert_helper sx t1 t2 ->
-  be_typing C [::BI_cvtop t1 CVO_convert t2 sx] (Tf [::T_num t2] [::T_num t1])
-| bet_reinterpret : forall C t1 t2, t1 <> t2 -> (tnum_length t1) = (tnum_length t2) ->
-  be_typing C [::BI_cvtop t1 CVO_reinterpret t2 None] (Tf [::T_num t2] [::T_num t1])
+| bet_cvtop : forall C op t1 t2 sx,
+    cvtop_valid t2 op t1 sx ->
+    be_typing C [::BI_cvtop t2 op t1 sx] (Tf [::T_num t1] [::T_num t2])
 | bet_unreachable : forall C ts ts',
   be_typing C [::BI_unreachable] (Tf ts ts')
 | bet_nop : forall C, be_typing C [::BI_nop] (Tf [::] [::])
